{-

Facts about Rational Numbers

-}
{-# OPTIONS --safe #-}
module Classical.Preliminary.QuoQ where

open import Cubical.Foundations.Prelude
open import Cubical.Algebra.CommRing
open import Cubical.Algebra.RingSolver.Reflection

-- It seems there are bugs when applying ring solver to explicit ring.
-- The following is a work-around.
private
  module Helpers {â„“ : Level}(ğ“¡ : CommRing â„“) where
    open CommRingStr (ğ“¡ .snd)

    helper1 : (p q : ğ“¡ .fst) â†’ ((p + q) + (1r + 1r) Â· (- p)) â‰¡ q - p
    helper1 = solve ğ“¡

    helper2 : (p pâ»Â¹ qâ»Â¹ : ğ“¡ .fst) â†’ p Â· (pâ»Â¹ Â· qâ»Â¹) â‰¡ (p Â· pâ»Â¹) Â· qâ»Â¹
    helper2 = solve ğ“¡

    helper3 : (q pâ»Â¹ qâ»Â¹ : ğ“¡ .fst) â†’ q Â· (pâ»Â¹ Â· qâ»Â¹) â‰¡ (q Â· qâ»Â¹) Â· pâ»Â¹
    helper3 = solve ğ“¡


open import Cubical.Data.Sigma
open import Cubical.Data.Empty as Empty
open import Cubical.Data.NatPlusOne
open import Cubical.HITs.Rationals.QuoQ using (â„š)
open import Cubical.Algebra.Ring
open import Cubical.Relation.Nullary

open import Classical.Preliminary.QuoInt using (â„¤Order)
open import Classical.Preliminary.QuoQ.Base public
open import Classical.Preliminary.QuoQ.Field using (â„šField ; _/_ ; Â·-/-lInv) public
open import Classical.Preliminary.QuoQ.Order using (â„šOrder ; 1>0) public
open import Classical.Algebra.Field
open import Classical.Algebra.OrderedRing

private
  variable
    p q r s : â„š


{-

  The Ordering of â„š

-}

open FieldStr       â„šField
open OrderedRingStr â„šOrder

open Helpers (â„šOrder .fst)


2>0 : 2 > 0
2>0 = +-Pres>0 {x = 1} {y = 1} 1>0 1>0

-1<0 : - 1 < 0
-1<0 = -Reverse>0 {x = 1} 1>0

q+1>q : q + 1 > q
q+1>q {q = q} = +-rPosâ†’> {x = 1} {y = q} 1>0

q-1<q : q - 1 < q
q-1<q {q = q} = +-rNegâ†’< {x = - 1} {y = q} -1<0


middle : (p q : â„š) â†’ â„š
middle p q = (p + q) / 2

middle-sym : (p q : â„š) â†’ middle p q â‰¡ middle q p
middle-sym p q i = (+Comm p q i) / 2

2Â·middle : (p q : â„š) â†’ 2 Â· middle p q â‰¡ p + q
2Â·middle p q = Â·-/-lInv (p + q) 2

middle-l : (p q : â„š) â†’ 2 Â· (middle p q - p) â‰¡ q - p
middle-l p q = Â·Rdist+ 2 (middle p q) _ âˆ™ (Î» i â†’ 2Â·middle p q i + 2 Â· (- p)) âˆ™ helper1 p q

middle-r : (p q : â„š) â†’ 2 Â· (middle p q - q) â‰¡ p - q
middle-r p q = (Î» i â†’ 2 Â· (middle-sym p q i - q)) âˆ™ middle-l q p

middle>l : p < q â†’ middle p q > p
middle>l {p = p} {q = q} p<q =
  Diff>0â†’> {x = middle p q} {y = p} (Â·-rPosCancel>0 {x = 2} {y = middle p q - p} 2>0
    (subst (_> 0) (sym (middle-l p q)) (>â†’Diff>0 {x = q} {y = p} p<q)))

middle<r : p < q â†’ q > middle p q
middle<r {p = p} {q = q} p<q =
  Diff<0â†’< {x = middle p q} {y = q} (Â·-rPosCancel<0 {x = 2} {y = middle p q - q} 2>0
    (subst (_< 0) (sym (middle-r p q)) (<â†’Diff<0 {x = p} {y = q} p<q)))


p>0â†’pâ»Â¹>0 : (p>0 : p > 0) â†’ inv (>-arefl {x = p} p>0) > 0
p>0â†’pâ»Â¹>0 {p = p} p>0 = Â·-rPosCancel>0 {x = p} {y = inv (>-arefl {x = p} p>0)} p>0 pÂ·pâ»Â¹>0
  where pÂ·pâ»Â¹>0 : p Â· inv (>-arefl {x = p} p>0) > 0
        pÂ·pâ»Â¹>0 = subst (_> 0) (sym (Â·-rInv (>-arefl {x = p} p>0))) 1>0

p>q>0â†’pÂ·qâ»Â¹>1 : (q>0 : q > 0) â†’ p > q â†’ p Â· inv (>-arefl {x = q} q>0) > 1
p>q>0â†’pÂ·qâ»Â¹>1 {q = q} {p = p} q>0 p>q =
  subst (p Â· inv (>-arefl {x = q} q>0) >_) (Â·-rInv (>-arefl {x = q} q>0))
    (Â·-rPosPres< {x = inv (>-arefl {x = q} q>0)} {y = q} {z = p} (p>0â†’pâ»Â¹>0 {p = q} q>0) p>q)

inv-Reverse< : (p>0 : p > 0)(q>0 : q > 0) â†’ p > q â†’ inv (>-arefl {x = p} p>0) < inv (>-arefl {x = q} q>0)
inv-Reverse< {p = p} {q = q} p>0 q>0 p>q = qâ»Â¹>pâ»Â¹
  where pâ‰¢0 = >-arefl {x = p} p>0
        qâ‰¢0 = >-arefl {x = q} q>0
        pâ»Â¹ = inv pâ‰¢0
        qâ»Â¹ = inv qâ‰¢0
        pâ»Â¹Â·qâ»Â¹>0 : pâ»Â¹ Â· qâ»Â¹ > 0
        pâ»Â¹Â·qâ»Â¹>0 = Â·-Pres>0 {x = pâ»Â¹} {y = qâ»Â¹} (p>0â†’pâ»Â¹>0 {p = p} p>0) (p>0â†’pâ»Â¹>0 {p = q} q>0)
        pÂ·pâ»Â¹Â·qâ»Â¹>qÂ·qâ»Â¹Â·pâ»Â¹ : (p Â· pâ»Â¹) Â· qâ»Â¹ > (q Â· qâ»Â¹) Â· pâ»Â¹
        pÂ·pâ»Â¹Â·qâ»Â¹>qÂ·qâ»Â¹Â·pâ»Â¹ = transport (Î» i â†’ helper2 p pâ»Â¹ qâ»Â¹ i > helper3 q pâ»Â¹ qâ»Â¹ i)
          (Â·-rPosPres< {x = pâ»Â¹ Â· qâ»Â¹} {y = q} {z = p} pâ»Â¹Â·qâ»Â¹>0 p>q)
        1Â·qâ»Â¹>1Â·pâ»Â¹ : 1 Â· qâ»Â¹ > 1 Â· pâ»Â¹
        1Â·qâ»Â¹>1Â·pâ»Â¹ = transport (Î» i â†’ Â·-rInv pâ‰¢0 i Â· qâ»Â¹ > Â·-rInv qâ‰¢0 i Â· pâ»Â¹) pÂ·pâ»Â¹Â·qâ»Â¹>qÂ·qâ»Â¹Â·pâ»Â¹
        qâ»Â¹>pâ»Â¹ : qâ»Â¹ > pâ»Â¹
        qâ»Â¹>pâ»Â¹ = transport (Î» i â†’ Â·Lid qâ»Â¹ i > Â·Lid pâ»Â¹ i) 1Â·qâ»Â¹>1Â·pâ»Â¹
